% !TeX root = ../main.tex

\chapter{Model Hamiltonians}

\section{Hierarchy of Hamiltonians}

For solids like
\[\cdots ~ \circ ~ \circ ~ \circ ~ \circ ~ \circ ~ \circ ~ \cdots\]
$\sum_i N(R_i) \to$ periodic potential ($\leftarrow$ single electron $\leftrightarrow quantum geroetry \to $ phonons).

$h_0 \xrightarrow{a\to0}\pdif x \to k(-\infty,+\infty) \in (-\frac\pi a,\frac\pi a) \to$ MÃ³ire $N l m$

\section{Pariser-Parr-Pople Model (tight-binding + interaction)}

\subsection{Hydrogen molecule}

For two hydrogen atoms
\begin{center}
\begin{tikzpicture}
  \draw (-1,-1) cos (0,0) sin (1,1) cos (2,0) sin (3,-1) ;
\end{tikzpicture}
\end{center}
\[h_0 = (-\frac{\nabla_x^2}{2m}),~ \nu(x_1,x_2)\]
\[h_0 = \sum_{1,2,...,n} \hat n_i(\epsilon_n^0) \epsilon_N^0 \to \epsilon(\hat n_1 + \hat n_2)
  + \sum_{\sigma,\sigma',nm}T_{1n}(R) (d_{1n\sigma}\dagger d_2n\sigma + d_{2M_\sigma'}d_{M_\sigma})\]
$\ket|\varphi_1^n>$, $\ket|\varphi_2^n>$. $\braket<\varphi_1^n|n_0|\varphi_2^m>$.

$h_\text{int} = v(\hat n_{1\uparrow}n_{1\downarrow} + \hat n_{2\uparrow}n_{2\downarrow}) + \nu_{12}(\hat n_1 - 1)(\hat n_2 - 1)$.

\section{Ammonia \ce{NH3}}

\section{Bloch electrons in 2nd Quantization}

Single particle basis: Bloch state $\ket|\bm k\sigma>$. Wave function $\braket<\bm r|\bm k\sigma> = \psi_{\bm k\sigma}(\bm r)$, $\psi_k = u_k(r)\upe^{\iu\bm k\cdot r}$

For single particle Hamiltonian
\begin{equation}
    \mathcal H_0 =  \sum_{\substack{k,\sigma\\k',\sigma'}}
                      \braket<k\sigma|h_0|k'\sigma'>d_k^\dagger d_{k'\sigma'}
    \Rightarrow \sum_{k\sigma} \epsilon(k) d_{k\sigma}^\dagger d_{k\sigma}
\end{equation}
For tight-binding $\sum_{ij}t_{ij} \ketbra|i><j| $
\begin{equation}
  H_0 = \sum_{\substack{\sigma\sigma'\\ij}}
        T_{ij\sigma\sigma'}\hat d^\dagger_{i\sigma}\hat d_{j\sigma'}
\end{equation}
\begin{equation}
  \braket<r|\bm k\sigma> \Leftrightarrow \braket<r|i\sigma>
\end{equation}
which is called \emph{(Maximally-localized) Wannier function}: exponentially atomic.

\subsection{Generic lattice}

The hamiltonian
\begin{equation}
  \mathcal H_0 = \sum_{ij} t_{ij} c_{i\sigma}\dagger c_{j\sigma} + \sum_i \epsilon_0 c_i^\dagger c_i,~
  H = \sum_k c_{k\alpha}^\dagger H_{\alpha\beta}\hat C_{k\beta},~
  \hat C_k = \frac1{\sqrt N} \sum_{i,\alpha} \upe^{-\iu \bm k (\bm R + \bm b_\alpha)} \hat c_{i, \bm b\alpha}
\end{equation}
Here,
\[
  \bm R_{i,A} = \sum_{n_1,n_2} n_1 \bm a_1 + n_2 \bm a_2 + \bm b_A,~ \bm R_{i,B}
= \sum_{n_1,n_2} n_1 \bm a_1 + n_2\bm a_2 + \bm b_B,~ \bm b_A
= (a,0), ~ \bm b_B = (0,1)
\]
$\alpha,\beta$: sublattice, spins; orbitals index.

\subsection{Graphene}

\begin{equation}
  \bm  a_1 = \frac a2(3,\sqrt3), ~ \bm a_2 = \frac a2(3,-\sqrt3),~
  \bm b_B = a(1,0),~ \delta_1 = \bm a_1 + \bm b_B,~ \delta_2 = \frac a2(1 - \sqrt3),~ \delta_3 = a(1,0).
\end{equation}
\begin{equation}
  \mathcal H = -t\sum (a_i^\dagger b_j + \text{h.c.})
\end{equation}
while $a_i = C_{R_i,A}$, $b = C_{R_i,B}$, and $h_k \approx \sum_\delta \upe^{\iu k\delta} + \upe^{-\iu k\delta}$
Then
\[
  H =
  \begin{pmatrix}
    a_k^\dagger & b_k^\dagger
  \end{pmatrix}
  \begin{pmatrix}
    0 & h_k\\
    h_k & 0
  \end{pmatrix}
  \begin{pmatrix}
    a_k\\b_k
  \end{pmatrix}
\]

pumping: \tikz[baseline]{\draw (0,0) rectangle (1,1);}

\begin{equation}
  h_k = t \ab[\upe^{i(1,0) \cdot \bm k} + \upe^{-\iu(1,0) \cdot \bm k} + \upe^{\iu(0,1) \cdot \bm k} + \cdots] = -2t(\cos k_x + \cos k_y)
\end{equation}
and
\begin{equation}
  H_k = -\sum 2t(\cos k_x + \cos k_y) c_k^\dagger c_k
\end{equation}

$h_k$ near some point (Dirac point): $h_k \sim (\bm k - \bm K) \pdv{h_k}k$, so it can be written as $h_k \sim \bm v_F \cdot \delta \bm k \leftrightarrow \pdif{\bm x}$

\subsection{Flat-bannd}

$h_k = \text{const}$ now.

Landau levels

Landau gauge: 

Symmertic Gauge $\ket|\phi_{LG}> \Rightarrow \sum \ket|\Phi_{SG}>$

magnetic translation $T_x$, $T_y$: $a_x, a_y \propto \dot l_b$

\subsection{Electron phonon coupling: BCS}

Hamiltonian with solid:
\begin{equation}
  \mathcal H_\text{solid}
  \begin{cases}
    \mathcal H_\text{phono} = \sum_{\bm q} \mathcal E(\bm q) b_q^\dagger b_q\\
    \mathcal H_\text{Bloch} = \sum_k \mathcal E(k) c_k^\dagger c_k
  \end{cases}
\end{equation}

$V(R_i,x_i)$

\begin{equation}
  H_{e-p} = \sum_{k_1} \sum_{q \bm G} T (b_q^\dagger + b_{-q}^\dagger) \hat a_{k+q+\bm G}^\dagger \hat a_k
\end{equation}
\[
  \bar x_j^* = \frac1n \sum_{i=1}^n x_{ij} - \bar x_j
= \frac1n \ab(\sum_{i=1}^n x_{ij} - \sum_{i=1}^n \bar x_j)
\]

\section{QM identical partical}

\begin{enumerate}
  \item $\ket|1:\phi_1>$, $\ket|2:\chi_2>$ -> occupation num. of condition
  \begin{itemize}
    \item $\ket|n_{\phi_1}, n_{\chi_2}>$
    in real space: $\phi \to \hat x$;
  \end{itemize}
  After interchange particle label, there should be a sign: $(\pm 1)^p$: minus - fermion; boson: trivial.
  so we have
  \[
    (-1)^p \leftrightarrow [d_n^\dagger, d_m]_\mp:
    d_n^\dagger d_m \mp d_m d_n^\dagger
  \]
  $[d_n, d_m]_\mp = 0 = [d_n^\dagger, d_m^\dagger]$.
  $d_n^\dagger d_m^\dagger \ket|0> = -d_m^\dagger d_n^\dagger \ket|0>$
\end{enumerate}

\section{Electron-phonon coupling}

$V_\text{ion-ion} = \sum V(R_i - R_j) \Rightarrow \sum_q \omega_q a_q^\dagger a_q$,

$V_\text{el-el} = \sum V(r_i - r_j) \Rightarrow \sum_i u n_{i\sigma} n_{iq} = + \cdots \sum_{ij} V n_i n_j$,

$V_\text{el-ion} = \sum V(R_i - r_j) \Rightarrow \sum_{\sigma q} (b_q^{-1} + b_{q-}) c_{k+q\sigma}^+ c_{k\sigma}$

corsplication: feed back effect (self-consistent eq.) == DFT


\hrule

\[
  H_{ep} = \sum_{kq\sigma}T_{kq} (b_q + \hat b_{-q})G_{k+q,\sigma}^\alpha a_{k\sigma}
\]
$MW_\text{ene}$-field BCS

\section{Effective$H_{a,g(\text{femons})}$}


\section{canonical transformaission}

Also called: Foldy-Wyen

\section{effection H canonical transf}

\[H = H_0 + \delta H\]
Broad prodive $\hat T = \upe^{-\hat{\mathcal S}} \mathcal H \upe^{\mathcal S}$.
Expand: \[
\tilde H = H + [H,\hat S]_- + \frac1{2!} [[\hat H,\hat S]_-S]_-
= H_0 + \delta H + [H_0,\hat S] + [\delta H, \hat S]
\]
find $\hat S: [H_0,\hat S] + \Delta H = 0$. S is usually called generator.

$\Rightarrow H_0 + [\Delta H, S] + \frac1{2!}[([H_0,S] + [\delta H,S]),S]
= H_0 + [\delta H, S] + \frac12 [-\delta H,S] + O(S^2) = H_0 + \frac12[\delta H,S]$

So, from $\delta H$ u get. $H = H_0 + \frac12[\delta H,S]$.

\section{For el-ph coupling $\mathsf{\hat S
  = \sum _{kq\sigma} \tau_q (x b_q + y b_{-q}^\dagger) a_{k+ q\sigma}^* a_k}$}
\[
  H_0 = \sum \epsilon_k a_{k\sigma}^\dagger a_{k\sigma}
\]
The commutator to $S$ is
\begin{align*}
  [H_0, \hat S] & = \sum \tau_q \{x(\epsilon(k+1) - \epsilon(k) - \hbar \omega_q)b_q + y(\epsilon(k+q) - \epsilon(k) + \hbar\omega_q) b_{-q}^\dagger\} a_{k+q\sigma}^\dagger a_{k\sigma}\\
& = -H_\text{el-ph} \Rightarrow
  \begin{cases}
    x = (\epsilon(k) - \epsilon(k+1) + \hbar (\omega)q^{-1})\\
    y = (\epsilon(k) - \epsilon(k+1) - \hbar (\omega)q^{-1})
  \end{cases}
\end{align*}
then, the effective Hamiltonian
\[
  H_\text{eff} = \frac12 [\delta H,\hat S]
= \frac12 \sum_{\substack{kk'\\q\sigma\sigma'}}
  \tau_{-q} \tau_q (q-x) a_{k+q}^\dagger a_{k'-q} a_{k'\sigma'} a_{k\sigma}
\]
$x = \frac{1}{\epsilon(k) - \epsilon(k+q) - \hbar\omega_q} \approx \delta(\epsilon(k) - \epsilon(k+1) - \hbar\omega_q)$.

Consider this $\delta$-function
\[
  \int \d E = \frac{1}{E \pm \hbar \omega_q} \delta(E - \hbar\omega_q)
\]
\[H_0 = \sum \epsilon_n a_n^\dagger a_n, \hat G = (E - H_0)^{-1} = G[E]\]
Green's function:
\[
  (E - H_{ph})^{-1} = G_{Phi}
\]
\[
  \tilde H = H_0 + H_{eff} = \sum_k \epsilon_k \tilde a_{k\sigma}^\dagger \tilde a_{k\sigma}
+ \frac12 \sum_{kk',q\sigma\sigma'} T_q T_{-q} (y-x) \tilde a_{k+q}^\dagger \tilde a_{k'-q}^\dagger \tilde a_{k'\sigma'} \tilde a_{k\sigma}
\]
\[\upe^{-\hat S} H_0 \upe^{\hat S} = \upe^{-S}a_k^\dagger (e^S e^{-S}) a_k \upe^{S}\]

\[
  \tilde a_k^\dagger = \upe^{-S} a_k^\dagger \upe^S = a^\dagger +
  [a_k^\dagger,S] + ... = a_k^\dagger + \sum_q (x
   b_q + y b_{-q})^\dagger,~
  \tilde a_k = \upe^S a_k \upe^{-S}
\]

\section{From el-ph to BCS}

at low-T, $k \in near ES$. $|T_q|^2(y - x) \sim < 0$, means for particular part of fermion, the attraction become attractive.
\[
  H = \sum_k \epsilon_k c_{k\sigma}^\dagger c_{k\sigma} - v \sum_{kk'} c_{k\uparrow}^+ c_{k\downarrow}^+ c_{k'\downarrow} c_{k'\uparrow}.
\]
This is called Richardson = RCS model Inone0meanfield
1. not a sc. qs => CFT
2. prove bcs, superconductivity spontuneous sym. treaking: add some like 
 Bogoliubov.

 Meanfield BCS model.

 SBB: $H_{GB} = \sum \epsilon_k c_{k\sigma}^\dagger c_{k\sigma}$
 
 \section{Holstein model}

 \begin{enumerate}
  \item $H_c = \sum_s \omega_0 (a_s^\dagger a_s + \frac12)$
  \item $H_\text{int} = -q \sum_{s\sigma} d_{s\sigma}^\dagger d_{s\sigma} (a_s + a_s^*)$
  \item $H_{el} = \sum_i (t_{ij} d_{is\sigma}^\dagger d_{js\sigma} + h.c.)$
  \item Strong compling limi. Leads to heavy poloron.
  \item Lang-Firsov transformation,(c.t.)
  \[
    \hat S = -\iu \frac g{\omega_0} \sum \hat n_{s\sigma} (a_s^\dagger - a_s)
  \]
  \[
    H_{cp} = T\sum (B_s^\dagger B_{{S}})
  \]
  $\hat B_s = \upe^{q/\omega_0}$
 \end{enumerate}

 \section{elec-el interaction}

 \[V_{el-el} = \sum V(r_i - r_j)\].

 \[
  \Rightarrow H_A = \sum \epsilon_k c_{k\sigma}^{-1} c_{k\sigma}
+ u \hat n_{d\uparrow}n_{d\downarrow} + \sum \epsilon_d d^\dagger d
+ V \sum k (c_{k\sigma}^\dagger d \sigma + d^\dagger \sigma c_{k\sigma})
\]
\[
 S = \sum_{k\sigma} (A_k c_{k\sigma}^\dagger d_\sigma - A_k d_\sigma^\dagger c_{k\sigma}) + \sum (B_A d_\sigma c_k^\dagger - B_k^\dagger c_{k\sigma d_\sigma^\dagger})
\]
\[
  A_K = \frac{V_k}{\epsilon_k - \epsilon d},~ B_k = \frac{V_k}{\epsilon_k - (\epsilon_d + b)}
\]
then
\[
 H_\text{eff} = \frac12 [\delta H, S] = \frac12 [\delta H, S(H_0)]
\]
while $H_0 = H_c + H_{n,d}$.
\[
  H_\text{eff} = J_k \bm S_d \cdot \bm S_{c,o}
= \sum_{kk'} J_{kk'} (\bm S_d \cdot \sum_{\alpha\beta} c_{k'\alpha}^\dagger \frac{\bm \sigma_{\alpha\beta}}2 c_{k\beta} + \frac14 \sum_\sigma c_{k'\sigma}^\dagger c_{k\sigma})
\]
\[
  \bm S_d = \sum_{\alpha\beta} \hat d_\alpha \frac{\sigma_{\alpha\beta}}{2} \hat d_\beta
\]
So, 
\[
  S_z = \frac12 (d_\uparrow^\dagger d_\uparrow
              - d_\downarrow^\dagger d_\downarrow),~
  S_z^+ =
  \begin{pmatrix}
    0 & 1\\0 & 0
  \end{pmatrix} = d_\uparrow^\dagger d_\downarrow,
  S^- =
  \begin{pmatrix}
    0 & 0\\1 & 0
  \end{pmatrix} = d_\downarrow^\dagger d_\uparrow
\]
\begin{framed}
  \[\text{Hkondo-imparity} = J_k \bm S_d \bm S_{c,o}\]
\end{framed}
for $J_K > 0$, $J_K = \frac{4V^2}{U}$.

After the treatment, from anderson module to kondo modo:
\[
  H_{And} \to H_{Kondo m} = \sum \epsilon_k c_k^\dagger c_k + J_k \bm S_\alpha \cdot \bm S_{c,N}
\]
$S_d$ is free moment, formation of a local moment.

$J_k$ can become negative, so change the kondo limit, Anti FM -- compling,
to becoma a FM.

\section{Hubbard model}

\begin{equation}
  H = \sum_{\sigma k} \epsilon_k c_{k\sigma}^\dagger c_{k\sigma} + N \sum_i (n_\uparrow -\frac12)(n_\downarrow -\frac12) + (\sum_{\sigma k} -\mu c_{k\sigma}^\dagger c_{k\sigma})
= -\sum_{ij\sigma} t_{ij} c_{i\sigma}^\dagger c_{j\sigma}
\end{equation}

\subsection{Schrieff-Wolff transformation (C.T.)}

For $n = 1$, deal with Heisenberg model
\begin{equation}
  H_{Heis} = \sum_{ij} J_{ij} \bm S_i \bm S_j
\end{equation}
while $J_{ij} = \frac{4t_{ij} t_{ji}}N = \frac{4t^2}{N}$.

When doping, $t-J$ model
\[
  H = \sum_{ij} t_{ij} \tilde{c_{ik}} \tilde c_{j\sigma} + \sum J \bm S_{i} \cdot \bm S_j.
\]
so-called Ggutzwillen projection, project out double-occupancy.

Gutzwiller approximation $\delta \sum t \hat c_i^\dagger c_{j\sigma} + \sum J(1 - 2\delta) \bm S_i \cdot \bm S_j$.

\section{Many layers of QMB problems}

\begin{enumerate}
  \item reduce degrees of freedom
    (wrong way: CT, quasi particles; polaron)
  \item methods to reduce DoF: link/crosscheck different methods
  path tn: Effective theory EFT.
\end{enumerate}
